feat: `ObjectProp`

LeanPy/Data/Object/Basic.lean
@@ -43,10 +43,6 @@ instance {self : Object} : LawfulTypeRef self.ty := self.lawful_ty
 
 namespace Object
 
-@[inline] def getData
-  [Nonempty α] [TypeName α] (self : Object) (h : self.data.kind = typeName α)
-: α := self.data.get h
-
 theorem eq_iff (self other : Object) :
   self = other ↔
   self.id = other.id ∧ self.ty = other.ty ∧ self.data = other.data
@@ -54,6 +50,14 @@ theorem eq_iff (self other : Object) :
   let {lawful_slots := h1, ..} := self
   let {lawful_slots := h2, ..} := other
   simp [mk'.injEq, ← TypeSlotsRef.ty_inj, h1, h2]
+
+theorem lawful_subobject
+  {self : Object} (h : self.ty ⊆ ty) : ty.IsValidObject self.id self.data
+:= self.ty.isValidObject_mro self.lawful_object h
+
+@[inline] def getData
+  [Nonempty α] [TypeName α] (self : Object) (h : self.data.kind = typeName α)
+: α := self.data.get h
 
 /--
 Returns whether this object is the constant `None`.
@@ -70,7 +74,6 @@ Equivalent to the Python `self is not None`.
 -/
 @[inline] def isNotNone (self : Object) : Bool :=
   self.id != .none
-
 
 /--
 Returns whether this object is the `True` singleton.
@@ -98,89 +101,110 @@ This is equivalent to the Python `self is True or self is False`.
 
 end Object
 
-/-! ## TypeProp -/
+/-! ## ObjectProp -/
 
 /--
-A predicate about a type.
-Used to encode Python type relations in Lean types.
--/
-abbrev TypeProp := TypeRef → Prop
+A predicate about an object.
 
-def TypeProp.Any : TypeProp :=
+Alternatively, this can be interpreted as the set of satisfying objects.
+-/
+abbrev ObjectProp := Object → Prop
+
+namespace ObjectProp
+
+def Any : ObjectProp :=
   fun _ => True
 
-def TypeProp.Subtype (p : TypeProp) (ty : TypeRef) : TypeProp :=
-  fun t => p t ∧ t ⊆ ty
+def ofRaw (p : Raw) : ObjectProp :=
+  fun self => p self.id self.data
 
-theorem TypeProp.Subtype.property (h : Subtype p ty t) : p t :=
+instance : Coe Raw ObjectProp := ⟨.ofRaw⟩
+
+def And (p q : ObjectProp) : ObjectProp :=
+  fun self => p self ∧ q self
+
+theorem And.property (h : And p q o) : p o :=
   h.1
 
-theorem TypeProp.Subtype.ty_subset (h : Subtype p ty t) : t ⊆ ty :=
+/-- Holds if the object satisfying `p` is a non-virtual instance of `ty`. -/
+def AndInstance (ty : TypeRef) (p : ObjectProp) : ObjectProp :=
+  p.And (·.ty ⊆ ty)
+
+theorem AndInstance.ty_subset (h : AndInstance ty p o) : o.ty ⊆ ty :=
   h.2
 
-theorem TypeProp.Subtype.trans (h : ty₁ ⊆ ty₂) (h₁ : Subtype p ty₁ t) : Subtype p ty₂ t :=
-  ⟨h₁.1, .trans h₁.2 h⟩
+theorem AndInstance.trans
+  (h : sub ⊆ sup) (h₁ : AndInstance sub p o)
+: AndInstance sup p o := ⟨h₁.1, .trans h₁.2 h⟩
+
+end ObjectProp
 
 /-! ## Object Subtypes -/
 
-structure PObject (p : TypeProp) extends Object where
-  inner_property : p ty
+structure PObject (p : ObjectProp) extends Object where
+  inner_property : p toObject
 
-theorem PObject.property (self : PObject p) : p self.ty :=
-  self.inner_property
+/-- An object which satisfies `p` and whose type is a subtype of `ty`, -/
+abbrev PSubObject (p : ObjectProp) (ty : TypeRef) :=
+  PObject (p.AndInstance ty)
+
+/--
+An object which satisfies `p` and whose type is a subtype of `subTy`,
+which is a subtype of `superTy`.
+-/
+abbrev PSubSubObject (p : ObjectProp) (subTy superTy : TypeRef) :=
+  PSubObject (p.AndInstance subTy) superTy
+
+abbrev SubObject (ty : TypeRef) := PSubObject .Any ty
+
+namespace Object
+
+@[inline] def cast (self : Object) (h : p self) : PObject p :=
+  ⟨self, h⟩
+
+@[inline] def toPObject (self : Object) : PObject .Any :=
+  self.cast .intro
+
+/-- Casts `self` to an instance of `ty`. -/
+@[inline] def asSubObject (self : Object) (h : self.ty ⊆ ty) : SubObject ty :=
+  self.cast ⟨.intro, h⟩
+
+/-- Casts `self` to an instance of its own type. -/
+@[inline] def toSubObject (self : Object) : SubObject self.ty :=
+  self.asSubObject .rfl
+
+end Object
+
+namespace PObject
 
 instance : CoeOut (PObject p) Object :=
   ⟨PObject.toObject⟩
 
-@[inline] def Object.cast (self : Object) (h : p self.ty) : PObject p :=
-  ⟨self, h⟩
+theorem property (self : PObject p) : p self :=
+  self.inner_property
 
-/-- An object whose type satisfies `p` and is a subtype of `ty`, -/
-abbrev PSubObject (p : TypeProp) (ty : TypeRef) :=
-  PObject (p.Subtype ty)
-
-/--
-An object whose type satisfies `p` and is a subtype of `subTy`,
-which is a subtype of `superTy`.
--/
-abbrev PSubSubObject (p : TypeProp) (subTy superTy : TypeRef) :=
-  PSubObject (p.Subtype subTy) superTy
-
-abbrev SubObject (ty : TypeRef) := PSubObject .Any ty
-
-@[inline] def Object.toPObject (self : Object) : PObject .Any :=
-  self.cast .intro
-
-@[inline] def Object.downcast (self : Object) (h : self.ty ⊆ ty) : SubObject ty :=
-  self.cast ⟨.intro, h⟩
-
-@[inline] def Object.toSubObject (self : Object) : SubObject self.ty :=
-  self.downcast .rfl
-
-@[inline] def PObject.upcast
+@[inline] def upcast
   (self : PSubObject p subTy) (h : subTy ⊆ superTy)
 : PSubSubObject p subTy superTy :=
   self.cast ⟨self.property, .trans self.property.2 h⟩
 
-theorem PObject.ty_subset {self : PSubObject p ty} : self.ty ⊆ ty :=
+theorem ty_subset {self : PSubObject p ty} : self.ty ⊆ ty :=
   self.property.ty_subset
 
-theorem Object.lawful_subobject
-  {self : Object} (h : self.ty ⊆ ty) : ty.IsValidObject self.id self.data
-:= self.ty.isValidObject_mro self.lawful_object h
-
-theorem PObject.lawful_subobject
+theorem lawful_subobject
   {self : PSubObject p ty} : ty.data.IsValidObject self.id self.data
 := self.toObject.lawful_subobject self.property.ty_subset
 
-theorem PObject.toObject_inj {self other : PObject p} :
+theorem toObject_inj {self other : PObject p} :
   self.toObject = other.toObject ↔ self = other
 := by cases self; cases other; simp
 
-theorem PObject.eq_iff {self other : PObject p} :
+theorem eq_iff {self other : PObject p} :
   self = other ↔
   self.id = other.id ∧ self.ty = other.ty ∧ self.data = other.data
 := by simp [← toObject_inj, Object.eq_iff]
+
+end PObject
 
 /-! ## Object Constructor -/
 
@@ -198,7 +222,6 @@ def TypeRef.mkObject
   lawful_bool := h_bool
   lawful_object := h
 }
-
 
 /-! `PyM` -/
 
